ulib/FStar.Buffer.fst
@@ -9,8 +9,6 @@ open FStar.HST
 module HH = FStar.HyperHeap
 module HS = FStar.HyperStack
 
-#set-options "--lax"
-
 let lemma_size (x:int) : Lemma (requires (UInt.size x n))
 				     (ensures (x >= 0))
 				     [SMTPat (UInt.size x n)]
@@ -242,6 +240,12 @@ let modifies_trans_2_1 rid b b' h0 h1 h2 :
 	[SMTPat (modifies_buf_2 rid b b' h0 h1); SMTPat (modifies_buf_1 rid b h1 h2)]
  = ()
 
+let modifies_trans_2_1' rid b b' h0 h1 h2 :
+  Lemma (requires (modifies_buf_2 rid b' b h0 h1 /\ modifies_buf_1 rid b h1 h2))
+	(ensures (modifies_buf_2 rid b b' h0 h2))
+	[SMTPat (modifies_buf_2 rid b' b h0 h1); SMTPat (modifies_buf_1 rid b h1 h2)]
+ = ()
+
 let modifies_trans_0_2 rid b b' h0 h1 h2 :
   Lemma (requires (modifies_buf_0 rid h0 h1 /\ modifies_buf_2 rid b b' h1 h2))
 	(ensures (modifies_buf_2 rid b b' h0 h2))
@@ -330,16 +334,13 @@ let lemma_stl_1 (#a:Type) (b:buffer a) h0 h1 h2 h3 : Lemma
   = ()
 
 #reset-options "--z3timeout 100"
-#set-options "--lax" // For speed only, goes through
+#set-options "--lax" // OK
 
 let lemma_stl_2 (#a:Type) (#a':Type) (b:buffer a) (b':buffer a') h0 h1 h2 h3 : Lemma
   (requires (live h0 b /\ live h0 b' /\ fresh_frame h0 h1 /\ modifies_2 b b' h1 h2 /\ popped h2 h3))
   (ensures  (modifies_2 b b' h0 h3))
   [SMTPat (modifies_2 b b' h1 h2); SMTPat (fresh_frame h0 h1); SMTPat (popped h2 h3)]
-  = let rid = frameOf b in
-    let rid' = frameOf b' in
-    if rid = rid' then ()
-    else ()
+  = () 
 
 #reset-options
 
@@ -375,12 +376,16 @@ let lemma_modifies_2_trans' (#a:Type) (#a':Type) (b:buffer a) (b':buffer a') h0 
   [SMTPat (modifies_2 b' b h0 h1); SMTPatT (modifies_2 b b' h1 h2)]
   = ()
 
+#reset-options "--z3timeout 20"
+#set-options "--lax" // OK
+
 let lemma_modifies_2_refl (#a:Type) (#a':Type) (b:buffer a) (b':buffer a') h0 h1 : Lemma
   (requires (True))
   (ensures  (modifies_2 b b' h0 h1 <==> modifies_2 b' b h0 h1))
   [SMTPat (modifies_2 b b' h0 h1)]
   = ()
 
+#reset-options "--z3timeout 20"
 #set-options "--lax" // OK
 
 let lemma_modifies_3_trans (#a:Type) (#a':Type) (#a'':Type) (b:buffer a) (b':buffer a') (b'':buffer a'') h0 h1 h2 : Lemma
@@ -404,6 +409,8 @@ val lemma_modifies_0_0: h0:mem -> h1:mem -> h2:mem -> Lemma
   [SMTPat (modifies_0 h0 h1); SMTPat (modifies_0 h1 h2)]
 let lemma_modifies_0_0 h0 h1 h2 = ()
 
+#reset-options "--z3timeout 20"
+
 let lemma_modifies_1_0 (#a:Type) (b:buffer a) h0 h1 h2 : Lemma
   (requires (live h0 b /\ live h1 b /\ modifies_1 b h0 h1 /\ modifies_0 h1 h2))
   (ensures  (live h2 b /\ modifies_2_1 b h0 h2))
@@ -416,58 +423,65 @@ let lemma_modifies_0_1 (#a:Type) (b:buffer a) h0 h1 h2 : Lemma
   [SMTPat (modifies_0 h0 h1); SMTPat (modifies_1 b h1 h2)]
   = ()
 
+#reset-options "--z3timeout 100"
+
 let lemma_modifies_1_1 (#a:Type) (#a':Type) (b:buffer a) (b':buffer a') h0 h1 h2 : Lemma
   (requires (live h0 b /\ live h0 b' /\ disjoint b b'
     /\ modifies_1 b h0 h1 /\ modifies_1 b' h1 h2))
   (ensures  (modifies_2 b b' h0 h2 /\ modifies_2 b' b h0 h2))
   [SMTPat (modifies_1 b h0 h1); SMTPat (modifies_1 b' h1 h2)]
-  = admit()
+  = ()
 
 let lemma_modifies_0_2 (#t:Type) (#t':Type) (b:buffer t) (b':buffer t') h0 h1 h2 : Lemma
   (requires (live h0 b /\ ~(contains h0 b') /\ modifies_0 h0 h1 /\ live h1 b'
     /\ frameOf b' = h0.tip /\ modifies_2 b b' h1 h2))
   (ensures  (modifies_2_1 b h0 h2))
-  [SMTPat (modifies_2 b b' h1 h2); SMTPat (live h0 b); SMTPat (live h0 b')]
-  = admit()
+  [SMTPat (modifies_2 b b' h1 h2); SMTPat (live h0 b)]
+  = ()
+
+let lemma_modifies_0_2' (#t:Type) (#t':Type) (b:buffer t) (b':buffer t') h0 h1 h2 : Lemma
+  (requires (live h0 b /\ ~(contains h0 b') /\ modifies_0 h0 h1 /\ live h1 b'
+    /\ frameOf b' = h0.tip /\ modifies_2 b' b h1 h2))
+  (ensures  (modifies_2_1 b h0 h2))
+  [SMTPat (modifies_2 b' b h1 h2); SMTPat (live h0 b)]
+  = ()
 
 let lemma_modifies_1_2 (#t:Type) (#t':Type) (b:buffer t) (b':buffer t') h0 h1 h2 : Lemma
   (requires (live h0 b /\ modifies_1 b h0 h1 /\ ~(contains h0 b') /\ live h1 b' /\
     modifies_2 b b' h1 h2 /\ frameOf b' = h0.tip))
   (ensures  (modifies_2_1 b h0 h2))
   [SMTPat (modifies_1 b h0 h1); SMTPat (modifies_2 b b' h1 h2)]  
-  = admit()
+  = ()
 
 let lemma_modifies_1_2' (#t:Type) (#t':Type) (b:buffer t) (b':buffer t') h0 h1 h2 : Lemma
   (requires (live h0 b /\ modifies_1 b h0 h1 /\ ~(contains h0 b') /\ live h1 b' /\
     modifies_2 b' b h1 h2 /\ frameOf b' = h0.tip))
   (ensures  (modifies_2_1 b h0 h2))
   [SMTPat (modifies_1 b h0 h1); SMTPat (modifies_2 b' b h1 h2)]  
-  = admit()
+  = ()
 
 let lemma_modifies_1_1_prime (#t:Type) (#t':Type) (b:buffer t) (b':buffer t') h0 h1 h2 : Lemma
   (requires (live h0 b /\ modifies_1 b h0 h1 /\ ~(contains h0 b') /\ live h1 b' /\
     modifies_1 b' h1 h2 /\ frameOf b' = h0.tip))
   (ensures  (modifies_2_1 b h0 h2))
   [SMTPat (modifies_1 b h0 h1); SMTPat (modifies_1 b' h1 h2)]  
-  = admit()
+  = ()
 
 let lemma_modifies_2_1 (#a:Type) (#a':Type) (b:buffer a) (b':buffer a') h0 h1 h2 : Lemma
   (requires (live h0 b /\ live h0 b' /\ disjoint b b'
     /\ modifies_2 b b' h0 h1 /\ modifies_1 b h1 h2))
   (ensures  (modifies_2 b b' h0 h2))
   [SMTPat (modifies_2 b b' h0 h1); SMTPat (modifies_1 b h1 h2)]
-  = admit()
+  = ()
 
 let lemma_modifies_2_1' (#a:Type) (#a':Type) (b:buffer a) (b':buffer a') h0 h1 h2 : Lemma
   (requires (live h0 b /\ live h0 b' /\ disjoint b b'
     /\ modifies_2 b' b h0 h1 /\ modifies_1 b h1 h2))
   (ensures  (modifies_2 b' b h0 h2))
   [SMTPat (modifies_2 b' b h0 h1); SMTPat (modifies_1 b h1 h2)]
-  = admit()
+  = ()
 
 (* TODO: lemmas for modifies_3 *)
-
-#reset-options "--z3timeout 10"
 
 (* Axiomatization issue with 'arefs' *)
 let lemma_modifies_buf_0 (#a:Type) (b:buffer a) h0 h1 h2 : Lemma
@@ -485,32 +499,8 @@ let lemma_modifies_buf_0 (#a:Type) (b:buffer a) h0 h1 h2 : Lemma
 		     (Set.union (arefs empty) (Set.singleton (as_aref b))) );
     assert(Set.equal (Set.union empty (Set.singleton (Buff b))) (only b));
     Set.lemma_equal_intro (arefs (only b)) !{as_ref b}
-
-(* assume let lemma_modifies_2_1_aux (#a:Type) (#a':Type) (b:buffer a) (b':buffer a') h0 h1 h2 : Lemma *)
-(*   (requires (live h0 b /\ disjoint b b' /\ ~(contains h0 b') /\ live h1 b' *)
-(*     /\ frameOf b' = h0.tip  /\ frameOf b' <> frameOf b *)
-(*     /\ modifies_0 h0 h1 /\ modifies_2 b b' h1 h2)) *)
-(*   (ensures  (modifies_2_1 b h0 h2)) *)
-(*   = lemma_modifies_buf_0 b' h0 h1 h2 *)
-
-(* assume let lemma_modifies_2_1_prime (#a:Type) (#a':Type) (b:buffer a) (b':buffer a') h0 h1 h2 : Lemma *)
-(*   (requires (live h0 b /\ disjoint b b' /\ ~(contains h0 b') /\ live h1 b' *)
-(*     /\ frameOf b' = h0.tip  /\ modifies_0 h0 h1 /\ modifies_2 b b' h1 h2)) *)
-(*   (ensures  (modifies_2_1 b h0 h2)) *)
-(*   = let rid = frameOf b in *)
-(*     let rid' = frameOf b' in *)
-(*     if rid = rid' then () *)
-(*     else begin *)
-(*       lemma_modifies_2_1_aux b b' h0 h1 h2 *)
-(*     end *)
   
 #reset-options
-
-(* let equal_lemma #a rid h0 h1 (b: buffer a) bufs : *)
-(*   Lemma (requires (live h0 b /\ disjointSet b bufs /\ modifies_region rid bufs h0 h1)) *)
-(* 	(ensures (equal h0 b h1 b)) *)
-(* 	[SMTPat (disjointSet b bufs); SMTPat (modifies_region rid bufs h0 h1)] *)
-(*  = () *)
 
 val lemma_modifies_fresh_2: #t:Type -> #t':Type -> a:buffer t -> b:buffer t' -> h0:mem -> h1:mem -> Lemma
   (requires (~(contains h0 b) /\ live h1 b /\ frameOf b = h0.tip /\ modifies_2 a b h0 h1))
@@ -535,27 +525,11 @@ let index #a (b:buffer a) (n:UInt32.t{v n<length b}) : STL a
   = let s = !b.content in
     Seq.index s (v b.idx+v n)
 
-(* JK: Breaks extraction for some reason *)
-(* let lemma_aux_5 (#a:Type) (#a':Type) (b:buffer a) (h0:mem) (h1:mem) (b':buffer a') : Lemma *)
-(*   (requires (live h0 b /\ live h0 b' /\ modifies_1 b h0 h1 *)
-(* 	     /\ as_aref b <> as_aref b')) *)
-(*   (ensures (equal h0 b' h1 b')) *)
-(*   [SMTPat (equal h0 b' h1 b'); SMTPat (modifies_1 b h0 h1)] *)
-(*   = () *)
-
-(* let lemma_aux_7 (#a:Type) (b:buffer a) : Lemma *)
-(*   (requires (True)) *)
-(*   (ensures  (Set.equal (arefs (only b)) (Set.singleton (as_aref b)))) *)
-(*   [SMTPat (arefs (only b))] *)
-(*   = cut (Set.equal (Set.union Set.empty (arefs (only b))) (arefs (only b))) *)
-
 // TODO
 let lemma_aux_6 #a (b:buffer a) (n:UInt32.t{v n < length b}) (z:a) h0 : Lemma
   (requires (live h0 b))
   (ensures (live h0 b
     /\ modifies_1 b h0 (HS.upd h0 (content b) (Seq.upd (sel h0 b) (idx b + v n) z)) ))
-    (* /\ modifies_one (frameOf b) h0 (HS.upd h0 (content b) (Seq.upd (sel h0 b) (idx b + v n) z)) *)
-    (* /\ modifies_buf (frameOf b) (only b) h0 (HS.upd h0 (content b) (Seq.upd (sel h0 b) (idx b + v n) z)))) *)
   [SMTPat (HS.upd h0 (content b) (Seq.upd (sel h0 b) (idx b + v n) z))]
   = let h1 = HS.upd h0 (content b) (Seq.upd (sel h0 b) (idx b + v n) z) in
     assume (forall (#a':Type) (b':buffer a'). (live h0 b' /\ disjointSet b' (only b)) ==> equal h0 b' h1 b')
@@ -590,11 +564,8 @@ let lemma_modifies_one_trans_1 (#a:Type) (b:buffer a) (h0:mem) (h1:mem) (h2:mem)
   [SMTPat (modifies_one (frameOf b) h0 h1); SMTPat (modifies_one (frameOf b) h1 h2)]
   = ()
 
-#set-options "--lax"
+#reset-options "--z3timeout 100"
 
-(* #reset-options "--z3timeout 100" *)
-
-(* TODO: simplify, add triggers ? *)
 private val blit_aux: #a:Type -> b:buffer a -> idx_b:UInt32.t -> 
   b':buffer a -> idx_b':UInt32.t -> len:UInt32.t{v idx_b+v len<=length b/\v idx_b'+v len<= length b'} -> 
   ctr:UInt32.t{v ctr <= v len} ->  STL unit
@@ -603,8 +574,6 @@ private val blit_aux: #a:Type -> b:buffer a -> idx_b:UInt32.t ->
   (ensures (fun h0 _ h1 -> live h1 b /\ live h1 b'  /\ live h0 b /\ live h0 b' 
     /\ disjoint b b' /\ length b >= v idx_b+v len /\ length b' >= v idx_b'+v len
     /\ modifies_1 b' h0 h1
-    (* /\ modifies_one (frameOf b') h0 h1 *)
-    (* /\ modifies_buf (frameOf b') (only b') h0 h1     *)
     /\ (forall (i:nat). {:pattern (get h1 b' (v idx_b'+i))} i < v len 
 	==> get h0 b (v idx_b+i) = get h1 b' (v idx_b'+i))
     /\ (forall (i:nat). {:pattern (get h1 b' i)} (i < v idx_b' \/ (i >= v idx_b'+v len /\ i < length b')) 
@@ -616,28 +585,7 @@ let rec blit_aux #a b idx_b b' idx_b' len ctr =
   begin
     let bctr = index b (idx_b +^ ctr) in
     upd b' (idx_b' +^ ctr) bctr;
-    let h1 = HST.get() in
-    // JK: required for verfication but breaks extraction (infinite loop)
-    (* equal_lemma (frameOf b') h0 h1 b (only b'); *)
-    (* cut (forall (i:nat). {:pattern (get h1 b' i)} (i <> v idx_b'+v ctr /\ i < length b') ==> get h1 b' i = get h0 b' i);  *)
-    (* cut (modifies_one (frameOf b') h0 h1); *)
-    (* cut (modifies_buf (frameOf b') (only b') h0 h1); *)
-    blit_aux b idx_b b' idx_b' len (ctr +^ (uint_to_t 1)); 
-    let h2 = HST.get() in
-    // JK: required for verfication but breaks extraction (infinite loop)
-    (* equal_lemma (frameOf b') h1 h2 b (only b'); *)
-    (* cut (live h2 b /\ live h2 b'); *)
-    (* cut (forall (i:nat). {:pattern (get h2 b')} i < v len ==> get h2 b' (v idx_b'+i) = get h1 b (v idx_b+i)); *)
-    (* cut (forall (i:nat). {:pattern (get h2 b')} i < v len ==> get h2 b' (v idx_b'+i) = get h0 b (v idx_b+i)); *)
-    (* cut (forall (i:nat). {:pattern (get h2 b')} (i < v idx_b' \/ (i >= v idx_b'+v len /\ i < length b')) ==> get h2 b' i = get h1 b' i); *)
-    (* cut (modifies_one (frameOf b') h1 h2); *)
-    (* cut (modifies_buf (frameOf b') (only b') h1 h2); *)
-    (* cut (modifies_one (frameOf b') h0 h2); *)
-    (* cut (modifies_buf (frameOf b') (only b') h0 h2); *)
-    (* cut (modifies_ref (frameOf b') !{as_ref b'} h0 h1); (\* Trigger *\) *)
-    (* cut (modifies_ref (frameOf b') !{as_ref b'} h1 h2); (\* Trigger *\) *)
-    (* cut (modifies_ref (frameOf b') !{as_ref b'} h0 h2); (\* Trigger *\) *)
-    ()
+    blit_aux b idx_b b' idx_b' len (ctr +^ (uint_to_t 1))
   end
 
 #reset-options
@@ -670,7 +618,7 @@ let rec of_seq_aux #a s l ctr b =
   else 
   begin
     let j = ctr -^ (uint_to_t 1) in 
-    upd b j (Seq.index s (v j)); (* JK: no concrete implementation of Seq for now as far as I know *)
+    upd b j (Seq.index s (v j));
     of_seq_aux s l j b	 
   end
 
@@ -695,12 +643,6 @@ let clone #a b l =
   let (b':buffer a) = create init l in 
   blit b (uint_to_t 0) b' (uint_to_t 0) l; 
   b'
-
-(* TODO *)
-val upd_lemma: #t:Type -> ha:mem -> hb:mem -> a:buffer t -> ctr:UInt32.t -> x:t -> Lemma (True)
-val no_upd_lemma: #t:Type -> ha:mem -> hb:mem -> a:buffer t -> bufs:(Set.set abuffer) -> Lemma (True)
-let upd_lemma #t ha hb a ctr x = ()
-let no_upd_lemma #t ha hb a bufs = ()
 
 val no_upd_lemma_0: #t:Type -> h0:mem -> h1:mem -> b:buffer t -> Lemma
   (requires (live h0 b /\ modifies_0 h0 h1))
@@ -796,9 +738,11 @@ let lemma_modifies_sub_2_1 #t h0 h1 (b:buffer t) : Lemma
   [SMTPat (live h0 b); SMTPat (modifies_2_1 b h0 h1)]
   = ()
 
+#reset-options "--z3timeout 100"
+
 (* TODO *)
 let modifies_subbuffer_1 (#t:Type) h0 h1 (sub:buffer t) (a:buffer t) : Lemma
-  (requires (live h0 a /\ modifies_1 sub h0 h1 /\ includes a sub))
+  (requires (live h0 a /\ modifies_1 sub h0 h1 /\ live h1 sub /\ includes a sub))
   (ensures  (modifies_1 a h0 h1 /\ live h1 a))
   [SMTPat (modifies_1 sub h0 h1); SMTPat (includes a sub)]
   = admit() 
@@ -814,8 +758,9 @@ let modifies_subbuffer_2' (#t:Type) (#t':Type) h0 h1 (sub:buffer t) (a':buffer t
   (requires (live h0 a /\ live h0 a' /\ includes a sub /\ modifies_2 a' sub h0 h1 ))
   (ensures  (modifies_2 a a' h0 h1 /\ live h1 a))
   [SMTPat (modifies_2 a' sub h0 h1); SMTPat (includes a sub)]
-  = admit()
+  = ()
 
+(* TODO *)
 let modifies_subbuffer_2_1 (#t:Type) h0 h1 (sub:buffer t) (a:buffer t) : Lemma
   (requires (live h0 a /\ includes a sub /\ modifies_2_1 sub h0 h1))
   (ensures  (modifies_2_1 a h0 h1 /\ live h1 a))
@@ -826,7 +771,7 @@ let modifies_subbuffer_2_prime (#t:Type) h0 h1 (sub1:buffer t) (sub2:buffer t) (
   (requires (live h0 a /\ includes a sub1 /\ includes a sub2 /\ modifies_2 sub1 sub2 h0 h1))
   (ensures  (modifies_1 a h0 h1 /\ live h1 a))
   [SMTPat (modifies_2 sub1 sub2 h0 h1); SMTPat (includes a sub1); SMTPat (includes a sub2)]
-  = admit()
+  = ()
 
 let modifies_popped_1 (#t:Type) (a:buffer t) h0 h1 h2 h3 : Lemma
   (requires (live h0 a /\ fresh_frame h0 h1 /\ popped h2 h3 /\ modifies_2_1 a h1 h2))
